fixed composition

src/subgroup/composition.lean
@@ -13,8 +13,8 @@ def group.nontrivial (G : Type) [group G] : Prop := (⊥ : subgroup G) ≠ ⊤
   group.nontrivial G ↔ (⊥ : subgroup G) ≠ ⊤ := iff.rfl
 
 -- Some lemmas about pushing top and bot over isomorphisms
-lemma subgroup.iso_bot_eq_bot {G H : Type} [group G] [group H] 
-  (φ : G ≅ H) : subgroup.map φ.1 (⊥ : subgroup G) = (⊥ : subgroup H) := 
+lemma subgroup.map_bot_eq_bot {G H : Type} [group G] [group H] 
+  (φ : G →* H) : subgroup.map φ (⊥ : subgroup G) = (⊥ : subgroup H) := 
 begin
   ext, rw [mem_map, mem_bot_iff],
   split, 
@@ -35,13 +35,14 @@ begin
   rw ← subgroup.closure_le, simp,
 end
 
-lemma subgroup.iso_top_eq_top {G H : Type} [group G] [group H] 
-  (φ : G ≅ H) : subgroup.map φ.1 (⊤ : subgroup G) = (⊤ : subgroup H) := 
+lemma subgroup.map_top_eq_top {G H : Type} [group G] [group H] 
+  (φ : G →* H) (hφ : surjective φ) : 
+  subgroup.map φ (⊤ : subgroup G) = (⊤ : subgroup H) := 
 begin
   ext, split; intro,
     { exact subgroup.mem_top _ },
     { rw mem_map,
-      rcases φ.2.2 x with ⟨x, rfl⟩,
+      rcases hφ x with ⟨x, rfl⟩,
       refine ⟨x, subgroup.mem_top _, rfl⟩ }
 end
 
@@ -51,11 +52,19 @@ lemma subgroup.nontrivial_of_iso_nontrivial {G H : Type} [group G] [group H]
 begin
   intros hG h,
   apply hG, 
-  rw [← subgroup.iso_top_eq_top (iso_symm φ),
-      ← subgroup.iso_bot_eq_bot (iso_symm φ), h],
+  rw [← subgroup.map_top_eq_top (iso_symm φ).1 (iso_symm φ).2.2,
+      ← subgroup.map_bot_eq_bot (iso_symm φ).1, h],
 end
 
-namespace normal
+/-- Everything is in top -/
+lemma normal.mem_top {G : Type} [group G] (g : G) : g ∈ (⊤ : normal G) :=
+begin
+  rw [← normal.mem_carrier, ← singleton_subset_iff],
+  change {g} ≤ ((⊤ : normal G) : set G),
+  rw ← normal.closure_le, simp,
+end
+
+namespace composition
 
 variables {G : Type} [group G]
 
@@ -71,34 +80,6 @@ variables {G : Type} [group G]
 -- def subgroup.normal_pair' (A B : subgroup G): Prop :=
 --   (monoid_hom.range (subgroup.le_hom (show A ⊓ B ≤ B, by exact inf_le_right))).normal
 
--- instance : has_top $ normal G := 
--- ⟨ { carrier := univ,
---     one_mem' := mem_univ _,
---     mul_mem' := λ _ _ _ _, mem_univ _,
---     inv_mem' := λ _ _, mem_univ _,
---     conj_mem' := λ _ _ _, mem_univ _ } ⟩
-
-/-- The normal subgroup of a normal subgroup induced by a smaller normal 
-  subgroup through the inclusion map -/
-def normal.𝒾 {G : Type} [group G] {A B : normal G} (hle : A ≤ B) : normal B :=
-{ carrier := { b | b.1 ∈ A },
-  one_mem' := A.one_mem',
-  mul_mem' := λ _ _ ha hb, A.mul_mem' ha hb,
-  inv_mem' := λ _ h, A.inv_mem' h,
-  conj_mem' := λ _ h _, A.conj_mem' _ h _ }
-
-lemma normal.mem_𝒾 {G : Type} [group G] {A B : normal G} (hle : A ≤ B) 
-  {g : G} (hg : g ∈ B) : (⟨g, hg⟩ : B) ∈ normal.𝒾 hle ↔ g ∈ A := iff.rfl
-
-lemma normal.inv_𝒾 {G : Type} [group G] {A B : normal G} (hle : A ≤ B) 
-  {g : G} (hg : g ∈ B) : (⟨g, hg⟩⁻¹ : B) = ⟨g⁻¹, B.inv_mem' hg⟩ := rfl
-
-lemma normal.mul_𝒾 {G : Type} [group G] {A B : normal G} (hle : A ≤ B) 
-  {g h : G} (hg : g ∈ B) (hh : h ∈ B) : 
-  (⟨g, hg⟩ : B) * (⟨h, hh⟩ : B) = ⟨g * h, B.mul_mem' hg hh⟩ := rfl
-
-attribute [simp] normal.mem_𝒾 normal.inv_𝒾 normal.mul_𝒾
-
 variables (H : subgroup G) (N : normal G)
 
 /-- A group is simple if and only if it is nontrivial and all its normal subgroups 
@@ -109,23 +90,36 @@ def is_simple (G : Type) [group G] :=
 @[simp] lemma is_simple_def (G : Type) [group G] : is_simple G ↔ 
   group.nontrivial G ∧ ∀ N : normal G, N = ⊥ ∨ N = ⊤ := iff.rfl
 
-def chain_prop (A B : normal G) : Prop :=
-  ∃ (hle : A ≤ B), is_simple $ B /ₘ (normal.𝒾 hle)
+lemma comap_eq_bot {G H : Type} [group G] [group H] {φ : G →* H} {N : normal H}
+  (h : normal.comap φ N = (⊥ : normal G)) (hsur : surjective φ) : N = ⊥ :=
+begin
+  rw eq_bot_iff at h ⊢,
+  intros n hn, erw normal.mem_carrier at hn ⊢,
+  rcases hsur n with ⟨x, rfl⟩,
+  rw ← normal.mem_comap at hn,
+  rw [normal.mem_bot_iff.1 (h hn), map_one],
+  exact (⊥ : normal H).one_mem'
+end
 
-@[simp] lemma chain_prop_def {A B : normal G} :
-  chain_prop A B ↔ 
-  ∃ (hle : A ≤ B), is_simple $ B /ₘ (normal.𝒾 hle) := iff.rfl
+lemma comap_eq_top {G H : Type} [group G] [group H] {φ : G →* H} {N : normal H}
+  (h : normal.comap φ N = (⊤ : normal G)) (hsur : surjective φ) : N = ⊤ :=
+begin
+  rw eq_top_iff at h ⊢,
+  intros n _, erw normal.mem_carrier,
+  rcases hsur n with ⟨x, rfl⟩,
+  exact(normal.mem_comap _).1 (h (normal.mem_top x))
+end
 
-instance normal.inhabited : inhabited $ normal G := ⟨ ⊥ ⟩
-
-/-- Chain is a nonempty list of normal subgroups such that subsequent subgroups 
-  satisfies `chain_prop`, and furthermore, it begins with bot and ends with top -/
-structure chain (G : Type) [group G] :=
-(carrier    : list (normal G))
-(nonempty   : carrier ≠ list.nil)
-(chain_prop : carrier.chain' chain_prop)
-(chain_head : carrier.head = ⊥)
-(chain_last : carrier.last nonempty = ⊤)
+/-- `is_simple` is a group property, that is, it translates over group 
+  isomorphisms -/
+lemma is_simple_of_iso {G H : Type} [group G] [group H] 
+  (φ : G ≅ H) : is_simple G → is_simple H :=
+begin
+  refine λ hG, ⟨subgroup.nontrivial_of_iso_nontrivial φ hG.1, _⟩,
+  intro N, rcases hG.2 (normal.comap φ.1 N) with hN | hN,
+    { left, exact comap_eq_bot hN φ.2.2 },
+    { right, exact comap_eq_top hN φ.2.2 }
+end
 
 /-- A normal subgroup is maximal if and only if the quotient group by it is 
   simple -/
@@ -165,57 +159,96 @@ begin
     { exact or.inl rfl }
 end
 
-/-- Everything is in top -/
-lemma mem_top {G : Type} [group G] (g : G) : g ∈ (⊤ : normal G) :=
-begin
-  rw [← mem_carrier, ← singleton_subset_iff],
-  change {g} ≤ ((⊤ : normal G) : set G),
-  rw ← normal.closure_le, simp,
-end
+def is_conj_mem (A B : subgroup G) : Prop := ∀ a ∈ A, ∀ g ∈ B, g * a * g⁻¹ ∈ A
+
+@[simp] lemma is_conj_mem_def (A B : subgroup G) :
+  is_conj_mem A B ↔ ∀ a ∈ A, ∀ g ∈ B, g * a * g⁻¹ ∈ A := iff.rfl
+
+def normal.𝒾 {G : Type} [group G] {A B : subgroup G} (hle : A ≤ B) 
+  (h : is_conj_mem A B) : normal B :=
+{ carrier := { a | a.1 ∈ A },
+  one_mem' := A.one_mem',
+  mul_mem' := λ _ _ ha hb, A.mul_mem' ha hb,
+  inv_mem' := λ _ h, A.inv_mem' h,
+  conj_mem' := λ _ hs x, h _ hs _ x.2 }
+
+lemma normal.mem_𝒾 {G : Type} [group G] {A B : subgroup G} (hle : A ≤ B) 
+  (h : is_conj_mem A B) {g : G} (hg : g ∈ B) : 
+  (⟨g, hg⟩ : B) ∈ normal.𝒾 hle h ↔ g ∈ A := iff.rfl
+
+lemma normal.inclusion_inv {G : Type} [group G] {A B : subgroup G} (hle : A ≤ B) 
+  {g : G} (hg : g ∈ B) : (⟨g, hg⟩⁻¹ : B) = ⟨g⁻¹, B.inv_mem' hg⟩ := rfl
+
+lemma normal.inclusion_mul {G : Type} [group G] {A B : subgroup G} (hle : A ≤ B) 
+  {g h : G} (hg : g ∈ B) (hh : h ∈ B) : 
+  (⟨g, hg⟩ : B) * (⟨h, hh⟩ : B) = ⟨g * h, B.mul_mem' hg hh⟩ := rfl
+
+attribute [simp] normal.mem_𝒾 normal.inclusion_inv normal.inclusion_mul
+
+-- `chain_prop A B` means `∀ a ∈ A, g ∈ B, g * a * g⁻¹ ∈ A` 
+def chain_prop (A B : subgroup G) : Prop := 
+  ∃ (hle : A ≤ B) (H : is_conj_mem A B), is_simple $ B /ₘ (normal.𝒾 hle H)
+
+@[simp] lemma chain_prop_def {A B : subgroup G} :
+  chain_prop A B ↔ 
+  ∃ (hle : A ≤ B) (H : is_conj_mem A B), is_simple $ B /ₘ (normal.𝒾 hle H) := iff.rfl
+
+-- def chain_prop (A B : normal G) : Prop :=
+--   ∃ (hle : A ≤ B), is_simple $ B /ₘ (normal.𝒾 hle)
+
+-- @[simp] lemma chain_prop_def {A B : normal G} :
+--   chain_prop A B ↔ 
+--   ∃ (hle : A ≤ B), is_simple $ B /ₘ (normal.𝒾 hle) := iff.rfl
+
+instance normal.inhabited : inhabited $ subgroup G := ⟨ ⊥ ⟩
+
+/-- Chain is a nonempty list of subgroups such that subsequent subgroups 
+  satisfies `chain_prop`, and furthermore, it begins with bot and ends with top -/
+structure chain (G : Type) [group G] :=
+(carrier    : list (subgroup G))
+(nonempty   : carrier ≠ list.nil)
+(chain_prop : carrier.chain' chain_prop)
+(chain_head : carrier.head = ⊥)
+(chain_last : carrier.last nonempty = ⊤)
+
+lemma is_conj_mem_bot : is_conj_mem H ⊥ := λ _ _ _ hg, by simpa [mem_bot_iff.1 hg]
+
+lemma is_conj_mem_bot' : is_conj_mem ⊥ H := λ _ ha _ _,
+  by simp [mem_bot_iff.1 ha, one_mem]
+
+def to_top : G →* (⊤ : subgroup G) := ⟨λ g, ⟨g, subgroup.mem_top _⟩, by tidy⟩
+def to_top_iso : G ≅ (⊤ : subgroup G) := ⟨to_top, by tidy⟩
 
 def top_div_bot_iso : 
-  G ≅ (⊤ : normal G) /ₘ (@normal.𝒾 _ _ ⊥ (⊤ : normal G) le_top) :=
-{ to_fun := λ g, quotient.mk (@normal.𝒾 _ _ ⊥ (⊤ : normal G) le_top) 
-    (⟨g, mem_top _⟩ : (⊤ : normal G)),
-  map_mul' := by tidy,
-  is_bijective := 
+  (⊤ : subgroup G) ≅ (⊤ : subgroup G) /ₘ (normal.𝒾 
+    (@le_top _ _ (⊥ : subgroup G)) (is_conj_mem_bot' _)) := 
+{ is_bijective := 
     begin
       refine ⟨_, by tidy⟩,
-      intros x₁ x₂ hx, dsimp at hx,
+      rintros ⟨x₁, _⟩ ⟨x₂, _⟩ hx, dsimp at hx,
       rw [← coe_eq_mk, ← coe_eq_mk, mk_eq'] at hx,
-      rw @normal.inv_𝒾 _ _ (⊥ : normal G) _ bot_le at hx,
-      erw @normal.mul_𝒾 _ _ (⊥ : normal G) _ bot_le at hx,
-      erw [normal.mem_𝒾, mem_bot_iff] at hx,
-      rw ← group.inv_eq_of_mul_eq_one hx,
+      rw @normal.inclusion_inv _ _ (⊥ : subgroup G) _ bot_le at hx,
+      erw @normal.inclusion_mul _ _ (⊥ : subgroup G) _ bot_le at hx,
+      erw [normal.mem_𝒾, mem_bot_iff] at hx, 
+      congr, rw ← group.inv_eq_of_mul_eq_one hx,
       exact group.inv_inv _,
-    end }
+    end .. 
+    quotient.mk (normal.𝒾 (@le_top _ _ (⊥ : subgroup G)) (is_conj_mem_bot' _)) }
 
-def to_top : G →* (⊤ : normal G) := ⟨λ g, ⟨g, mem_top _⟩, by tidy⟩
-def to_top_iso : G ≅ (⊤ : normal G) := ⟨to_top, by tidy⟩
+def top_div_bot_iso' : 
+  G ≅ (⊤ : subgroup G) /ₘ (normal.𝒾 
+    (@le_top _ _ (⊥ : subgroup G)) (is_conj_mem_bot' _)) := 
+  group_hom.iso_comp to_top_iso top_div_bot_iso
 
 def trivial_chain (h : is_simple G) : chain G := 
 { carrier := [⊥, ⊤],
   nonempty := by simp,
   chain_prop := 
     begin
-      simp, 
-      refine ⟨subgroup.nontrivial_of_iso_nontrivial (top_div_bot_iso) h.1, λ N, _⟩,
-      rcases h with ⟨h₁, h₂⟩,
-      cases h₂ (comap to_top_iso.1 (normal.comap (quotient.mk _) N)) with h h,
-        { left, rw eq_bot_iff at h ⊢,
-          intros x hx,
-          rcases exists_mk x with ⟨y, rfl⟩,
-          rcases to_top_iso.2.2 y with ⟨x, rfl⟩,
-          erw [mem_bot_iff, ← coe_one, mk_eq', group.one_inv, group.one_mul],
-          change to_top_iso.1 x ∈ _,
-          rw ← mem_comap, convert one_mem _, rw ← mem_bot_iff,
-          apply h, erw [mem_comap, mem_comap], exact hx },
-        { right, rw eq_top_iff at h ⊢,
-          intros x hx,
-          rcases exists_mk x with ⟨y, rfl⟩,
-          rcases to_top_iso.2.2 y with ⟨x, rfl⟩,
-          erw [coe_eq_mk, ← mem_comap, ← mem_comap],
-          refine h (mem_top _) }
+      simp only [and_true, is_simple_def, list.chain'_singleton,
+                 bot_le, chain_prop_def, exists_prop_of_true, ne.def, 
+                 list.chain'_cons, group.nontrivial_def],
+      exact ⟨is_conj_mem_bot' _, is_simple_of_iso top_div_bot_iso' h⟩, 
     end,
   chain_head := by simp,
   chain_last := by simp }
@@ -231,6 +264,6 @@ def trivial_chain (h : is_simple G) : chain G :=
 
 -- instance [fintype G] : inhabited $ chain G := ⟨ sorry ⟩
 
-end normal
+end composition
 
 end mygroup
